Hs/Algorithm/Soundness.lean
@@ -1,28 +1,87 @@
 import Hs.HsTerm
 import Hs.Algorithm
 import Hs.HsJudgment
-import Hs.Compile
+import Hs.CompileJ
 
 set_option maxHeartbeats 500000
 
-theorem compile_soudness :
+@[simp]
+abbrev KindLike : Term -> Prop
+| _ -k> _ => true
+| ★ => true
+| _ => false
+
+inductive HsKindLike : HsTerm -> Prop where
+| HsType : HsKindLike `★
+| HsArrK : HsKindLike k1 -> HsKindLike k2 -> HsKindLike (k1 `-k> k2)
+
+
+theorem compile_soundness_kinds :
+  HsKindLike t ->
+  τ = `□ ->
   (j : Γ ⊢s t : τ) ->
   compile Γ t τ j = .some t' ->
-  CompileJ .term Γ ⟨t, τ; j, t'⟩ := by
-intro j c;
-unfold compile at c; split at c;
+  CompileKind t t' := by
+intro h e j c;
+induction Γ, t, τ, j using compile.induct generalizing t'
+case _ =>
+  unfold compile at c; cases c;
+  apply CompileKind.type;
+case _ j1 j2 ih1 ih2 =>
+  unfold compile at c; simp at c;
+  rw[Option.bind_eq_some] at c;
+  cases c; case _ t1' c1 =>
+  cases c1; case _ c1 c =>
+  rw[Option.bind_eq_some] at c;
+  cases c; case _ t2' c2 =>
+  cases c2; case _ c2 t3 =>
+  cases t3; cases h;
+  case _ h1 h2 =>
+  apply CompileKind.arrowk;
+  apply ih1 h1 rfl c1;
+  apply ih2 h2 rfl c2;
+all_goals (cases h)
+all_goals try (cases e)
 case _ => sorry
 case _ => sorry
 case _ => sorry
 case _ => sorry
-case _ => sorry
-case _ => sorry
-case _ => sorry
-case _ => sorry
-case _ => sorry
-case _ => sorry
-case _ => sorry
-case _ => sorry
-case _ => sorry
-case _ => sorry
-case _ => sorry
+
+-- theorem compile_soudness :
+--   (j : Γ ⊢s t : τ) ->
+--   compile Γ t τ j = .some t' ->
+--   (∃ idx, CompileJ .kind Γ idx) ∨ (∃ idx, CompileJ .type Γ idx) ∨ (∃ idx, CompileJ .term Γ idx) := by
+-- intro j c;
+-- induction Γ, t, τ, j using compile.induct generalizing t' <;> (unfold compile at c; simp at c)
+-- case _ wf =>
+--   apply Or.inl;
+--   exists ⟨`★, `□; HsJudgment.ax wf, ★⟩
+--   apply CompileJ.type;
+-- case _ A B Aj Bj ih1 ih2 =>
+--   rw [Option.bind_eq_some] at c;
+--   cases c; case _ t1 c =>
+--   cases c; case _ c1 c2 =>
+--   rw [Option.bind_eq_some] at c2;
+--   cases c2; case _ t2 c2 =>
+--   cases c2; case _ c2 t3 =>
+--   cases t3;
+--   apply Or.inl; exists ⟨A `-k> B, `□; HsJudgment.arrowk Aj Bj, t1 -k> t2⟩
+--   apply CompileJ.arrowk
+--   case _ => have ih1' := ih1 c1; simp at ih1'; sorry
+--   sorry
+--   assumption
+--   assumption
+-- case _ j _ _ _ j1 j2 =>
+--   sorry
+-- case _ => sorry
+-- case _ => sorry
+-- case _ => sorry
+-- case _ => sorry
+-- case _ => sorry
+-- case _ => sorry
+-- case _ => sorry
+-- case _ => sorry
+-- case _ => sorry
+-- case _ => sorry
+-- case _ => sorry
+-- case _ => sorry
