Hs/Metatheory/Weaken.lean
@@ -3,7 +3,7 @@ import Hs.HsJudgment
 import SystemFD.Ctx
 import Hs.Metatheory.TypeMatch
 
-theorem rename_lift r (A : Frame HsTerm) :
+theorem hs_rename_lift r (A : Frame HsTerm) :
   (∀ x, (Γ d@ x).apply r.to = Δ d@ (r x)) ->
   ∀ x, ((A::Γ) d@ x).apply r.lift.to = (A.apply r.to::Δ) d@ (Ren.lift r x)
 := by
@@ -19,33 +19,33 @@ case _ x =>
   rw [<-h x, Frame.apply_compose, Frame.apply_compose]; simp
 
 @[simp]
-abbrev idx_ren (r : Ren) : HsJudgmentArgs v -> HsJudgmentArgs v :=
+abbrev hs_idx_ren (r : Ren) : HsJudgmentArgs v -> HsJudgmentArgs v :=
   match v with
   | .prf => λ (t, A) => ([r.to]t, [r.to]A)
   | .wf => λ () => ()
 
-def rename (r : Ren) : (v : JudgmentVariant) -> {idx : HsJudgmentArgs v} ->
+def hs_rename (r : Ren) : (v : JudgmentVariant) -> {idx : HsJudgmentArgs v} ->
   HsJudgment v Γ idx ->
   ⊢s Δ ->
   (∀ x, (Γ d@ x).apply r.to = Δ d@ (r x)) ->
-  HsJudgment v Δ (idx_ren r idx)
+  HsJudgment v Δ (hs_idx_ren r idx)
 | .prf, (t, τ) , j, wf, f => match j with
-  | .implicitAllI h1 h2 h3 => .implicitAllI sorry (rename r .prf h2 wf f) sorry
+  | .implicitAllI h1 h2 h3 => .implicitAllI sorry (hs_rename r .prf h2 wf f) sorry
   | .implicitAllE h1 h2 => sorry
-  | .implicitArrI h1 h2 h3 h4 => sorry -- .implicitArrI (rename r .prf h1 wf f) sorry sorry sorry
+  | .implicitArrI h1 h2 h3 h4 h5 => sorry -- .implicitArrI (hs_rename r .prf h1 wf f) sorry sorry sorry
   | .implicitArrE h1 h2 => sorry
   | .ax wf' => .ax wf
-  | .arrowk h1 h2 => .arrowk (rename r .prf h1 wf f) (rename r .prf h2 wf f)
+  | .arrowk h1 h2 => .arrowk (hs_rename r .prf h1 wf f) (hs_rename r .prf h2 wf f)
   | .appk h1 h2 =>
-    .appk (rename r .prf h1 wf f) (rename r .prf h2 wf f)
+    .appk (hs_rename r .prf h1 wf f) (hs_rename r .prf h2 wf f)
   | @HsJudgment.allt Γ A _ h1 h2 =>
-      .allt (rename r .prf h1 wf f) sorry
+      .allt (hs_rename r .prf h1 wf f) sorry
   | .arrow h1 h2  =>
-    .arrow (rename r .prf h1 wf f) sorry
-           -- (by have h' := rename r .prf h2 (.wfempty wf) (rename_lift r .empty f); rw[Subst.lift_lemma]; sorry)
-           -- (rename r .prf h2 (by sorry) (by sorry))
+    .arrow (hs_rename r .prf h1 wf f) sorry
+           -- (by have h' := hs_rename r .prf h2 (.wfempty wf) (hs_rename_lift r .empty f); rw[Subst.lift_lemma]; sorry)
+           -- (hs_rename r .prf h2 (by sorry) (by sorry))
   | .farrow h1 h3 h2  =>
-    .farrow (rename r .prf h1 wf f) sorry sorry
+    .farrow (hs_rename r .prf h1 wf f) sorry sorry
   | @HsJudgment.var Γ x T wf' h => .var wf (by
     have e := f x; unfold Frame.get_type at h;
     split at h;
@@ -66,35 +66,35 @@ def rename (r : Ren) : (v : JudgmentVariant) -> {idx : HsJudgmentArgs v} ->
     case _ => sorry
     case _ => sorry
     case _ => sorry)
-  | .lam h1 h2 h3 => .lam (rename r .prf h1 wf f) sorry (rename r .prf h3 wf f)
+  | .lam h1 h2 h3 => .lam (hs_rename r .prf h1 wf f) sorry (hs_rename r .prf h3 wf f)
   | .app h1 h2 h3 =>
-    .app (rename r .prf h1 wf f) (rename r .prf h2 wf f) (by rw [h3]; rw[<-Subst.lift_lemma]; sorry)
+    .app (hs_rename r .prf h1 wf f) (hs_rename r .prf h2 wf f) (by rw [h3]; rw[<-Subst.lift_lemma]; sorry)
   | .hslet h1 h2 h3 h4 =>
-    .hslet (rename r .prf h1 wf f) (rename r .prf h2 wf f) sorry (rename r .prf h4 wf f)
+    .hslet (hs_rename r .prf h1 wf f) (hs_rename r .prf h2 wf f) sorry (hs_rename r .prf h4 wf f)
   | .hsIte h1 h2 h3 h4 h5 h6 h7 h8 h9 h10 =>
-    .hsIte (rename r .prf h1 wf f) (rename r .prf h2 wf f) (rename r .prf h3 wf f) (rename r .prf h4 wf f)
-           (rename r .prf h5 wf f) (rename r .prf h6 wf f) sorry sorry (by sorry)  sorry
+    .hsIte (hs_rename r .prf h1 wf f) (hs_rename r .prf h2 wf f) (hs_rename r .prf h3 wf f) (hs_rename r .prf h4 wf f)
+           (hs_rename r .prf h5 wf f) (hs_rename r .prf h6 wf f) sorry sorry (by sorry)  sorry
 | .wf, () , j, wf, r => by simp; apply wf
 
 
-def weaken :
+def hs_weaken :
   ⊢s (f :: Γ) ->
   Γ ⊢s t : A ->
   (f::Γ) ⊢s ([S]t) : ([S]A)
-| wf , h => rename (λ x => x + 1) .prf h wf (by intro; rw [Subst.to_S]; simp)
+| wf , h => hs_rename (λ x => x + 1) .prf h wf (by intro; rw [Subst.to_S]; simp)
 
-def weaken_empty :
+def hs_weaken_empty :
   Γ ⊢s t : A ->
   (.empty::Γ) ⊢s ([S]t) : ([S]A)
- := λ x => weaken (.wfempty (hs_judgment_ctx_wf .prf x)) x
+ := λ x => hs_weaken (.wfempty (hs_judgment_ctx_wf .prf x)) x
 
-def weaken_type :
+def hs_weaken_type :
   Γ ⊢s T : `★ ->
   Γ ⊢s t : A ->
   (.type T::Γ) ⊢s ([S]t) : ([S]A)
-:= λ h1 h2 => weaken (.wftype h1 (hs_judgment_ctx_wf .prf h1)) h2
+:= λ h1 h2 => hs_weaken (.wftype h1 (hs_judgment_ctx_wf .prf h1)) h2
 
-def weaken_kind :
+def hs_weaken_kind :
   Γ ⊢s T : `□ ->
   Γ ⊢s t : A ->
   (.kind T::Γ) ⊢s ([S]t) : ([S]A)
@@ -105,55 +105,55 @@ def weaken_kind :
 --   Γ ⊢s t : A ->
 --   (.kind T::Γ) ⊢s ([S]t) : ([S]A)
 -- := by
--- intro j1 j2; apply rename _ j2
+-- intro j1 j2; apply hs_rename _ j2
 -- case _ => constructor; apply j1; apply hs_judgment_ctx_wf j1
 -- case _ => intro x; simp; rw [Subst.to_S]
 
-def weaken_datatype :
+def hs_weaken_datatype :
   Γ ⊢s T : `□ ->
   Γ ⊢s t : A ->
   (.datatype T::Γ) ⊢s ([S]t) : ([S]A)
 := sorry
 -- := by
--- intro j1 j2; apply rename _ j2
+-- intro j1 j2; apply hs_rename _ j2
 -- case _ => constructor; apply j1; apply hs_judgment_ctx_wf j1
 -- case _ => intro x; simp; rw [Subst.to_S]
 
-def weaken_ctor :
+def hs_weaken_ctor :
   Γ ⊢s T : `★ ->
   ValidHsCtorType Γ T ->
   Γ ⊢s t : A ->
   (.ctor T::Γ) ⊢s ([S]t) : ([S]A) := sorry
 -- := by
--- intro j1 j2 j3; apply rename _ j3
+-- intro j1 j2 j3; apply hs_rename _ j3
 -- case _ => constructor; apply j1; apply hs_judgment_ctx_wf j1; apply j2
 -- case _ => intro x; simp; rw [Subst.to_S]
 
-def weaken_opent :
+def hs_weaken_opent :
   Γ ⊢s T : `□ ->
   Γ ⊢s t : A ->
   (.opent T::Γ) ⊢s ([S]t) : ([S]A) := sorry
 -- := by
--- intro j1 j2; apply rename _ j2
+-- intro j1 j2; apply hs_rename _ j2
 -- case _ => constructor; apply j1; apply hs_judgment_ctx_wf j1
 -- case _ => intro x; simp; rw [Subst.to_S]
 
-def weaken_openm :
+def hs_weaken_openm :
   Γ ⊢s T : `★ ->
   Γ ⊢s t : A ->
   (.openm T::Γ) ⊢s ([S]t) : ([S]A) := sorry
 -- by
--- intro j1 j2; apply rename _ j2
+-- intro j1 j2; apply hs_rename _ j2
 -- case _ => constructor; apply j1; apply hs_judgment_ctx_wf j1
 -- case _ => intro x; simp; rw [Subst.to_S]
 
-def weaken_insttype :
+def hs_weaken_insttype :
   Γ ⊢s T : `★ ->
   ValidHsInstType Γ T ->
   Γ ⊢s t : A ->
   (.insttype T::Γ) ⊢s ([S]t) : ([S]A) := sorry
 -- := by
--- intro j1 j2 j3; apply rename _ j3
+-- intro j1 j2 j3; apply hs_rename _ j3
 -- case _ => constructor; apply j1; apply hs_judgment_ctx_wf j1; apply j2
 -- case _ => intro x; simp; rw [Subst.to_S]
 
@@ -163,13 +163,13 @@ def weaken_insttype :
 --   Γ ⊢s t : A ->
 --   (.inst #x b::Γ) ⊢s ([S]t) : ([S]A)
 -- := by
--- intro j1 j2 j3; apply rename _ j3
+-- intro j1 j2 j3; apply hs_rename _ j3
 -- case _ => constructor; apply j1; apply j2; apply hs_judgment_ctx_wf j2
 -- case _ => intro x; simp; rw [Subst.to_S]
 
-def weaken_term :
+def hs_weaken_term :
   Γ ⊢s T : `★ ->
   Γ ⊢s b : T ->
   Γ ⊢s t : A ->
   (.term T b::Γ) ⊢s ([S]t) : ([S]A)
-:= λ h1 h2 h3 => weaken (.wfterm h1 h2 (hs_judgment_ctx_wf .prf h1)) h3
+:= λ h1 h2 h3 => hs_weaken (.wfterm h1 h2 (hs_judgment_ctx_wf .prf h1)) h3
