Hs/Metatheory/TypeMatch.lean
@@ -3,7 +3,7 @@ import Hs.HsJudgment
 import SystemFD.Ctx
 
 
-theorem lift_subst_rename {Γ : Ctx HsTerm} (A : Frame HsTerm) :
+theorem hs_lift_subst_rename {Γ : Ctx HsTerm} (A : Frame HsTerm) :
   (∀ n y, σ n = .re y -> (Γ d@ n).apply σ = Δ d@ y) ->
   (∀ n y, ^σ n = .re y -> ((A :: Γ) d@ n).apply (^σ) = (A.apply σ :: Δ) d@ y)
 := by
@@ -22,7 +22,7 @@ case _ n =>
     rw [Frame.apply_compose]; simp; rw [<-h1]
     rw [Frame.apply_compose]
 
-theorem lift_subst_stable {σ : Subst HsTerm} (A : Frame HsTerm) :
+theorem hs_lift_subst_stable {σ : Subst HsTerm} (A : Frame HsTerm) :
   (∀ n, (Γ d@ n).is_stable -> ∃ y, σ n = .re y) ->
   (∀ n, ((A :: Γ) d@ n).is_stable → ∃ y, (^σ) n = .re y)
 := by
@@ -35,7 +35,7 @@ case _ n =>
   cases h1; case _ z h2 =>
     rw [h2]; simp
 
-theorem neutral_form_subst {t : HsTerm} (σ : Subst HsTerm) :
+theorem hs_neutral_form_subst {t : HsTerm} (σ : Subst HsTerm) :
   (σ x = .re y) ->
   t.neutral_form = .some (x, sp) ->
   ([σ]t).neutral_form = .some (y, List.map (λ (v, l) => (v, [σ]l)) sp)
@@ -61,7 +61,7 @@ case _ z =>
     subst e1; subst e2; simp
     rw [h1]; simp
 
-theorem valid_head_variable_subst test σtest :
+theorem hs_valid_head_variable_subst test σtest :
   (∀ n, test n -> ∃ y, σ n = .re y ∧ σtest y) ->
   HsValidHeadVariable A test ->
   HsValidHeadVariable ([σ]A) σtest
@@ -73,11 +73,11 @@ cases h1; case _ sp h1 =>
   have lem1 := q x h2
   cases lem1; case _ y lem1 =>
   cases lem1; case _ lem1 lem2 =>
-    replace h1 := neutral_form_subst σ lem1 (Eq.symm h1); simp at h1
+    replace h1 := hs_neutral_form_subst σ lem1 (Eq.symm h1); simp at h1
     exists y; rw [lem2]; simp
     rw [h1]; simp
 
-theorem valid_ctor_subst :
+theorem hs_valid_ctor_subst :
   (∀ n y, σ n = .re y -> (Γ d@ n).apply σ = Δ d@ y) ->
   (∀ n, Γ.is_stable n -> ∃ y, σ n = .re y) ->
   ValidHsCtorType Γ A ->
@@ -86,7 +86,7 @@ theorem valid_ctor_subst :
 intro h1 h2 j
 induction j generalizing Δ σ
 case refl R Γ j =>
-  constructor; apply valid_head_variable_subst Γ.is_datatype Δ.is_datatype _ j
+  constructor; apply hs_valid_head_variable_subst Γ.is_datatype Δ.is_datatype _ j
   intro n h3
   have lem1 := Frame.is_datatype_implies_is_stable h3
   replace h2 := h2 n lem1
@@ -98,25 +98,25 @@ case _ Γ A B j ih =>
   simp; apply ValidHsCtorType.arrow
   replace ih := @ih (^σ)
     (((Frame.empty).apply σ) :: Δ)
-    (lift_subst_rename (Frame.empty) h1)
-    (lift_subst_stable (Frame.empty) h2)
+    (hs_lift_subst_rename (Frame.empty) h1)
+    (hs_lift_subst_stable (Frame.empty) h2)
   simp at ih; apply ih
 case _ Γ A B j ih =>
   simp; apply ValidHsCtorType.farrow
   replace ih := @ih (^σ)
     (((Frame.empty).apply σ) :: Δ)
-    (lift_subst_rename (Frame.empty) h1)
-    (lift_subst_stable (Frame.empty) h2)
+    (hs_lift_subst_rename (Frame.empty) h1)
+    (hs_lift_subst_stable (Frame.empty) h2)
   simp at ih; apply ih
 case _ Γ A B j ih =>
   simp; apply ValidHsCtorType.all
   replace ih := @ih (^σ)
     (((Frame.kind A).apply σ) :: Δ)
-    (lift_subst_rename (Frame.kind A) h1)
-    (lift_subst_stable (Frame.kind A) h2)
+    (hs_lift_subst_rename (Frame.kind A) h1)
+    (hs_lift_subst_stable (Frame.kind A) h2)
   simp at ih; apply ih
 
-theorem valid_insttype_subst :
+theorem hs_valid_insttype_subst :
   (∀ n y, σ n = .re y -> (Γ d@ n).apply σ = Δ d@ y) ->
   (∀ n, Γ.is_stable n -> ∃ y, σ n = .re y) ->
   ValidHsInstType Γ A ->
@@ -125,7 +125,7 @@ theorem valid_insttype_subst :
 intro h1 h2 j
 induction j generalizing Δ σ
 case _ R Γ j =>
-  constructor; apply valid_head_variable_subst Γ.is_opent Δ.is_opent _ j
+  constructor; apply hs_valid_head_variable_subst Γ.is_opent Δ.is_opent _ j
   intro n h3
   have lem1 := Frame.is_opent_implies_is_stable h3
   replace h2 := h2 n lem1
@@ -137,26 +137,26 @@ case _ Γ A B j ih =>
   simp; apply ValidHsInstType.arrow
   replace ih := @ih (^σ)
     (((Frame.empty).apply σ) :: Δ)
-    (lift_subst_rename (Frame.empty) h1)
-    (lift_subst_stable (Frame.empty) h2)
+    (hs_lift_subst_rename (Frame.empty) h1)
+    (hs_lift_subst_stable (Frame.empty) h2)
   simp at ih; apply ih
 case _ Γ A B j ih =>
   simp; apply ValidHsInstType.farrow
   replace ih := @ih (^σ)
     (((Frame.empty).apply σ) :: Δ)
-    (lift_subst_rename (Frame.empty) h1)
-    (lift_subst_stable (Frame.empty) h2)
+    (hs_lift_subst_rename (Frame.empty) h1)
+    (hs_lift_subst_stable (Frame.empty) h2)
   simp at ih; apply ih
 
 case _ Γ A B j ih =>
   simp; apply ValidHsInstType.all
   replace ih := @ih (^σ)
     (((Frame.kind A).apply σ) :: Δ)
-    (lift_subst_rename (Frame.kind A) h1)
-    (lift_subst_stable (Frame.kind A) h2)
+    (hs_lift_subst_rename (Frame.kind A) h1)
+    (hs_lift_subst_stable (Frame.kind A) h2)
   simp at ih; apply ih
 
-theorem stable_type_match_subst :
+theorem hs_stable_type_match_subst :
   (∀ n y, σ n = .re y -> (Γ d@ n).apply σ = Δ d@ y) ->
   (∀ n, Γ.is_stable n -> ∃ y, σ n = .re y) ->
   StableHsTypeMatch Γ A B ->
@@ -165,7 +165,7 @@ theorem stable_type_match_subst :
 intro h1 h2 j
 induction j generalizing Δ σ
 case _ R Γ j =>
-  constructor; apply valid_head_variable_subst Γ.is_stable Δ.is_stable _ j
+  constructor; apply hs_valid_head_variable_subst Γ.is_stable Δ.is_stable _ j
   intro n h3; replace h2 := h2 n h3
   cases h2; case _ w h2 =>
     exists w; rw [h2]; simp
@@ -174,12 +174,12 @@ case _ R Γ j =>
 case _ R Γ A B j1 j2 ih =>
   replace ih := @ih (^σ)
     (((Frame.empty).apply σ) :: Δ)
-    (lift_subst_rename (Frame.empty) h1)
-    (lift_subst_stable (Frame.empty) h2)
+    (hs_lift_subst_rename (Frame.empty) h1)
+    (hs_lift_subst_stable (Frame.empty) h2)
   simp at ih;
   simp; constructor; simp
   case _ =>
-    apply valid_head_variable_subst Γ.is_stable Δ.is_stable _ j1
+    apply hs_valid_head_variable_subst Γ.is_stable Δ.is_stable _ j1
     intro n h3; replace h2 := h2 n h3
     cases h2; case _ w h2 =>
       exists w; rw [h2]; simp
@@ -189,12 +189,12 @@ case _ R Γ A B j1 j2 ih =>
 case _ R Γ A B j1 j2 ih =>
   replace ih := @ih (^σ)
     (((Frame.empty).apply σ) :: Δ)
-    (lift_subst_rename (Frame.empty) h1)
-    (lift_subst_stable (Frame.empty) h2)
+    (hs_lift_subst_rename (Frame.empty) h1)
+    (hs_lift_subst_stable (Frame.empty) h2)
   simp at ih;
   simp; constructor; simp
   case _ =>
-    apply valid_head_variable_subst Γ.is_stable Δ.is_stable _ j1
+    apply hs_valid_head_variable_subst Γ.is_stable Δ.is_stable _ j1
     intro n h3; replace h2 := h2 n h3
     cases h2; case _ w h2 =>
       exists w; rw [h2]; simp
@@ -204,12 +204,12 @@ case _ R Γ A B j1 j2 ih =>
 case _ R Γ A B j1 j2 ih =>
   replace ih := @ih (^σ)
     (((Frame.kind A).apply σ) :: Δ)
-    (lift_subst_rename (Frame.kind A) h1)
-    (lift_subst_stable (Frame.kind A) h2)
+    (hs_lift_subst_rename (Frame.kind A) h1)
+    (hs_lift_subst_stable (Frame.kind A) h2)
   simp at ih;
   simp; constructor; simp
   case _ =>
-    apply valid_head_variable_subst Γ.is_stable Δ.is_stable _ j1
+    apply hs_valid_head_variable_subst Γ.is_stable Δ.is_stable _ j1
     intro n h3; replace h2 := h2 n h3
     cases h2; case _ w h2 =>
       exists w; rw [h2]; simp
@@ -217,13 +217,13 @@ case _ R Γ A B j1 j2 ih =>
       simp at h3; apply h3
   case _ => simp; apply ih
 
-theorem stable_type_match_beta t :
+theorem hs_stable_type_match_beta t :
   ¬ f.is_stable ->
   StableHsTypeMatch (f :: Γ) A B ->
   StableHsTypeMatch Γ (A β[t]) (B β[t])
 := by
 intro j1 j2
-apply stable_type_match_subst _ _ j2
+apply hs_stable_type_match_subst _ _ j2
 case _ =>
   intro n y h
   cases n <;> simp at *
@@ -234,7 +234,7 @@ case _ =>
   rw [Frame.is_stable_stable] at h1
   rw [h1] at j1; injection j1
 
-theorem prefix_type_match_subst :
+theorem hs_prefix_type_match_subst :
   (∀ n y, σ n = .re y -> (Γ d@ n).apply σ = Δ d@ y) ->
   (∀ n, Γ.is_stable n -> ∃ y, σ n = .re y) ->
   PrefixHsTypeMatch Γ A B T ->
@@ -243,7 +243,7 @@ theorem prefix_type_match_subst :
 intro h1 h2 j
 induction j generalizing Δ σ
 case _ Γ B j =>
-  constructor; apply valid_head_variable_subst Γ.is_stable Δ.is_stable _ j
+  constructor; apply hs_valid_head_variable_subst Γ.is_stable Δ.is_stable _ j
   intro n h3; replace h2 := h2 n h3
   cases h2; case _ w h2 =>
     exists w; rw [h2]; simp
@@ -253,24 +253,24 @@ case _ Γ A B V T j ih =>
   simp; constructor; simp
   replace ih := @ih (^σ)
     (((Frame.empty).apply σ) :: Δ)
-    (lift_subst_rename (Frame.empty) h1)
-    (lift_subst_stable (Frame.empty) h2)
+    (hs_lift_subst_rename (Frame.empty) h1)
+    (hs_lift_subst_stable (Frame.empty) h2)
   simp at ih; apply ih
 case _ Γ A B V T j ih =>
   simp; constructor; simp
   replace ih := @ih (^σ)
     (((Frame.kind A).apply σ) :: Δ)
-    (lift_subst_rename (Frame.kind A) h1)
-    (lift_subst_stable (Frame.kind A) h2)
+    (hs_lift_subst_rename (Frame.kind A) h1)
+    (hs_lift_subst_stable (Frame.kind A) h2)
   simp at ih; apply ih
 
-theorem prefix_type_match_beta t :
+theorem hs_prefix_type_match_beta t :
   ¬ f.is_stable ->
   PrefixHsTypeMatch (f :: Γ) A B T ->
   PrefixHsTypeMatch Γ (A β[t]) (B β[t]) (T β[t])
 := by
 intro j1 j2
-apply prefix_type_match_subst _ _ j2
+apply hs_prefix_type_match_subst _ _ j2
 case _ =>
   intro n y h
   cases n <;> simp at *
@@ -281,7 +281,7 @@ case _ =>
   rw [Frame.is_stable_stable] at h1
   rw [h1] at j1; injection j1
 
-theorem no_infinite_terms_arrow σ :
+theorem hs_no_infinite_terms_arrow σ :
   ¬ ([σ](A -t> B) = B)
 := by
 intro h
@@ -292,13 +292,13 @@ case _ v t1 t2 ih1 ih2 =>
     subst h1; replace ih2 := @ih2 ([σ]A) (^σ)
     simp at ih2; apply ih2; simp at h2; rw [h2]
 
-theorem stable_type_match_refl_inversion :
+theorem hs_stable_type_match_refl_inversion :
   StableHsTypeMatch Γ A A ->
   HsValidHeadVariable A Γ.is_stable
 := by
 intro j; cases j <;> simp [*]
 
-theorem no_valid_head_variable_with_all :
+theorem hs_no_valid_head_variable_with_all :
   ¬ HsValidHeadVariable (`∀{A}B) test
 := by
 intro h; unfold HsValidHeadVariable at h
@@ -306,7 +306,7 @@ cases h; case _ x h =>
 cases h; case _ h1 h2 =>
   simp at h1
 
-theorem no_valid_head_variable_with_arrow :
+theorem hs_no_valid_head_variable_with_arrow :
   ¬ HsValidHeadVariable (A → B) test
 := by
 intro h; unfold HsValidHeadVariable at h
@@ -315,7 +315,7 @@ cases h; case _ h1 h2 =>
   simp at h1
 
 
-theorem prefix_type_match_forced_refl :
+theorem hs_prefix_type_match_forced_refl :
   HsValidHeadVariable A Γ.is_stable ->
   PrefixHsTypeMatch Γ A B T ->
   B = T
@@ -325,12 +325,12 @@ cases j2
 case _ => rfl
 case _ =>
   exfalso
-  apply no_valid_head_variable_with_arrow j1
+  apply hs_no_valid_head_variable_with_arrow j1
 case _ =>
   exfalso
-  apply no_valid_head_variable_with_all j1
+  apply hs_no_valid_head_variable_with_all j1
 
-theorem datatype_opent_distinct : ValidHsCtorType Γ T -> ValidHsInstType Γ T -> False := by
+theorem hs_datatype_opent_distinct : ValidHsCtorType Γ T -> ValidHsInstType Γ T -> False := by
 intros vctor vit;
 cases vctor;
 case refl h1 =>
@@ -356,4 +356,4 @@ all_goals (
     case _ h2 =>
     cases h2; case _ nf _ => cases nf
   case _ h2 =>
-    apply datatype_opent_distinct h1 h2)
+    apply hs_datatype_opent_distinct h1 h2)
